src/riscv/Utility/FreeMonad.v
@@ -77,6 +77,76 @@ Module free.
       Qed.
     End WithState.
 
+    Section WithStateAndAbort.
+      Context {state : Type}.
+      Context (interpret_action : forall a : action,
+                  state ->                       (* initial state *)
+                  (result a -> state -> Prop) -> (* postcondition if finished *)
+                  (state -> Prop) ->             (* postcondition if aborted *)
+                  Prop).
+      Section WithOutput.
+        Context {output} (postF : output -> state -> Prop) (postA : state -> Prop).
+        Definition interpret_body rec (a : free output) (s : state) : Prop :=
+          match a with
+          | ret x => postF x s
+          | act a k => interpret_action a s (fun r => rec (k r)) postA
+          end.
+        Fixpoint interpret_fix a := interpret_body interpret_fix a.
+      End WithOutput.
+
+      Definition interpret {output} a s postF postA := @interpret_fix output postF postA a s.
+
+      Lemma interpret_ret {T} (x : T) m postF postA : interpret (ret x) m postF postA = postF x m.
+      Proof. exact eq_refl. Qed.
+      Lemma interpret_act {T} a (k : _ -> free T) s postF postA
+        : interpret (act a k) s postF postA
+        = interpret_action a s (fun r s => interpret (k r) s postF postA) postA.
+      Proof. exact eq_refl. Qed.
+
+      Context (interpret_action_weaken_post :
+        forall a (postF1 postF2 : _ -> _ -> Prop) (postA1 postA2 : _ -> Prop),
+        (forall r s, postF1 r s -> postF2 r s) ->
+        (forall s, postA1 s -> postA2 s) ->
+        forall s, interpret_action a s postF1 postA1 -> interpret_action a s postF2 postA2).
+
+      Lemma interpret_weaken_post {T} (p : free T) s
+            (postF1 postF2 : _ -> _ -> Prop) (postA1 postA2 : _ -> Prop):
+        (forall r s, postF1 r s -> postF2 r s) ->
+        (forall s, postA1 s -> postA2 s) ->
+        interpret p s postF1 postA1 -> interpret p s postF2 postA2.
+      Proof.
+        revert dependent s; induction p. 2: firstorder eauto.
+        cbn. intros. eapply interpret_action_weaken_post.
+        - intros. eapply H; try eassumption. exact H3.
+        - eassumption.
+        - eassumption.
+      Qed.
+
+      Lemma interpret_bind {A B} s postF postA (a : free A) (b : A -> free B) :
+        interpret (bind a b) s postF postA <->
+        interpret a s (fun x s => interpret (b x) s postF postA) postA.
+      Proof.
+        revert postF; revert postA; revert b; revert B; revert s; induction a.
+        2: { intros. cbn. reflexivity. }
+        split; intros; eapply interpret_action_weaken_post; intros.
+        - eapply H. exact H1.
+        - exact H1.
+        - eauto.
+        - eapply H. exact H1.
+        - exact H1.
+        - eauto.
+      Qed.
+
+      Lemma interpret_bind_ex_mid {A B} m0 postF postA (a : free A) (b : A -> free B) :
+        interpret (bind a b) m0 postF postA <->
+        (exists mid, interpret a m0 mid postA /\ forall x m1, mid x m1 -> interpret (b x) m1 postF postA).
+      Proof.
+        rewrite interpret_bind.
+        split; [intros ? | intros (?&?&?)].
+        { exists (fun x m1 => interpret (b x) m1 postF postA); split; eauto. }
+        { eauto using interpret_weaken_post. }
+      Qed.
+    End WithStateAndAbort.
   End WithInterface.
   Global Arguments free : clear implicits.
 End free. Notation free := free.free.
